fixing #57 on more effects

examples/micro-benchmarks/AssumeRequires.fst
@@ -7,6 +7,16 @@ let well_typed o = admit ()
 val get : o:(option 'a) -> Pure 'a (Some? o) (fun x -> Some?.v o == x)
 let get (Some x) = x
 
+val get_div : o:(option 'a) -> Div 'a (Some? o) (fun x -> Some?.v o == x)
+let get_div (Some x) = x
+
 // Lemma works too
 val lem : o:(option unit) -> Lemma (requires (Some? o)) (ensures (Some?.v o == ()))
 let lem o = ()
+
+// Testing misc effects
+val get_ghost : o:(option 'a) -> Ghost 'a (Some? o) (fun x -> Some?.v o == x)
+let get_ghost (Some x) = x
+
+val get_exn : o:(option 'a) -> Exn 'a (Some? o) (fun x -> V (Some?.v o) == x)
+let get_exn (Some x) = x
