ulib/prims.fst
@@ -140,8 +140,9 @@ irreducible let labeled (r:range) (msg:string) (b:Type) = b
 
 (* PURE effect *)
 let pure_pre = Type0
-let pure_post (a:Type) = a -> GTot Type0
-let pure_wp   (a:Type) = pure_post a -> GTot pure_pre
+let pure_post' (a:Type) (pre:pure_pre) = (_:a{pre}) -> GTot Type0 // c.f. #57
+let pure_post  (a:Type) = pure_post' a True
+let pure_wp    (a:Type) = pure_post a -> GTot pure_pre
 
 assume type guard_free: Type0 -> Type0
 
@@ -185,7 +186,7 @@ total new_effect { (* The definition of the PURE effect is fixed; no user should
 
 // Note the type of post, which allows to assume the precondition
 // for the well-formedness of the postcondition. c.f. #57
-effect Pure (a:Type) (pre:pure_pre) (post:(_:a{pre}) -> GTot Type0) =
+effect Pure (a:Type) (pre:pure_pre) (post:pure_post' a pre) =
         PURE a
              (fun (p:pure_post a) -> pre /\ (forall (x:a). post x ==> p x)) // pure_wp
 effect Admit (a:Type) = PURE a (fun (p:pure_post a) -> True)
@@ -203,7 +204,7 @@ sub_effect
 (* The primitive effect GTot is definitionally equal to an instance of GHOST *)
 effect GTot (a:Type) = GHOST a (pure_null_wp a)
 (* #set-options "--print_universes --print_implicits --print_bound_var_types --debug Prims --debug_level Extreme" *)
-effect Ghost (a:Type) (pre:Type) (post:pure_post a) =
+effect Ghost (a:Type) (pre:Type) (post:pure_post' a pre) =
        GHOST a
            (fun (p:pure_post a) -> pre /\ (forall (x:a). post x ==> p x))
 
